Source/Definability.v
@@ -793,13 +793,15 @@ Proof.
     do 2![rewrite Intermediate.wfprog_defined_procedures //].
     by rewrite -domm_union mem_domm e.
   have Hatomic : Atomic (I.CS.sem (Intermediate.program_link p c)) by admit.
-  (* RB: TODO: Fold in new finite behavior prefixes.
+  set m' := finpref_trace m.
   have {Hbeh} [cs [cs' [Hcs Hstar]]] :
       exists cs cs',
         I.CS.initial_state (Intermediate.program_link p c) cs /\
-        Star (I.CS.sem (Intermediate.program_link p c)) cs m cs'.
+        Star (I.CS.sem (Intermediate.program_link p c)) cs m' cs'.
     case: b / Hbeh Hpre.
-      move=> cs beh Hcs Hbeh [beh' e]; subst beh.
+      move=> cs beh Hcs Hbeh Hprefix (* [beh' e]; subst beh. *).
+      (* TODO *) admit. admit.
+(*
       case/(state_behaves_app_inv Hatomic): Hbeh=> cs' [Hstar Hbeh'].
       by exists cs, cs'; split; eauto.
     (* Program goes wrong initially and produces empty trace.  Thus, any state
@@ -807,22 +809,22 @@ Proof.
     move=> _ [[ | | |beh'] //=]; case: m=> [|//] _.
     do 2![exists (I.CS.initial_machine_state (Intermediate.program_link p c))].
     split; try reflexivity; exact: star_refl.
-  have {cs cs' Hcs Hstar} wf_m : well_formed_trace intf m.
+*)
+  have {cs cs' Hcs Hstar} wf_m : well_formed_trace intf m'.
     have [mainP [_ [HmainP _]]] := Intermediate.cprog_main_existence Hclosed.
     have wf_p_c := Intermediate.linking_well_formedness wf_p wf_c Hlinkable.
     exact: intermediate_well_formed_trace Hstar Hcs HmainP wf_p_c.
   have := definability Hclosed_intf intf_main wf_m.
-  set back := (program_of_trace intf m) => Hback.
+  set back := (program_of_trace intf m') => Hback.
   exists (program_unlink (domm (Intermediate.prog_interface p)) back).
   exists (program_unlink (domm (Intermediate.prog_interface c)) back).
-  exists (Terminates m); split=> /=.
+  exists (Terminates m'); split=> /=.
     rewrite -[RHS](unionmK (Intermediate.prog_interface p) (Intermediate.prog_interface c)).
     by apply/eq_filterm=> ??; rewrite mem_domm.
   split.
     rewrite /intf unionmC; last by case: Hlinkable.
     rewrite -[RHS](unionmK (Intermediate.prog_interface c) (Intermediate.prog_interface p)).
     by apply/eq_filterm=> ??; rewrite mem_domm.
-  *)
   (* Needs properties about unlinking. *)
   admit.
 Admitted.
